Make another take on evaluate_Halt_FUNPOW_next
The new interference_implemented_def seems much better, but it's not
quite right because ffi_proj is only returning the oracle's ffi state:
it should be returning the observable trace instead.

examples/ag32/compilation/proofs/hello_ag32ProofScript.sml
@@ -108,41 +108,45 @@ val _ = temp_overload_on("read_ffi",
 val _ = temp_overload_on("nxt",
   ``λmc n ms. FUNPOW mc.target.next n ms``);
 
-val interfer_FUNPOW_next_def = Define`
-  interfer_FUNPOW_next record_ffi mc ms ⇔
-   (∀n k.
-     ∃k'. (mc.next_interfer n (FUNPOW mc.target.next (k+1) ms)
-           = FUNPOW mc.target.next (k' + k + 1) ms) ∧
-           (∀ffi. record_ffi (FUNPOW mc.target.next k ms) ffi ⇒
-                  record_ffi (FUNPOW mc.target.next (1 + k) ms) ffi ∧
-                  record_ffi (FUNPOW mc.target.next (k' + k + 1) ms) ffi)) ∧
-   (∀n k.
-     ∃k'. (mc.ccache_interfer n
-            (mc.target.get_reg (FUNPOW mc.target.next k ms) mc.ptr_reg,
-             mc.target.get_reg (FUNPOW mc.target.next k ms) mc.len_reg,
-             FUNPOW mc.target.next k ms)
-           = FUNPOW mc.target.next (k' + k) ms) ∧
-           (∀ffi. record_ffi (FUNPOW mc.target.next k ms) ffi ⇒
-                  record_ffi (FUNPOW mc.target.next (k' + k) ms) ffi)) ∧
-   (∀n i b k.
-     ∃k'. (mc.ffi_interfer n (i, b, FUNPOW mc.target.next k ms)
-           = FUNPOW mc.target.next (k' + k) ms) ∧
-          (∀ffi conf bytes.
-            record_ffi (FUNPOW mc.target.next k ms) ffi ∧
-            (read_ffi (FUNPOW mc.target.next k ms) mc = (SOME conf, SOME bytes))
-            ⇒
-            record_ffi (FUNPOW mc.target.next (k' + k) ms)
-            (ffi ++ (if EL i mc.ffi_names = "" then [] else [IO_event (EL i mc.ffi_names) conf (ZIP(bytes,b))]))))`;
+val interference_implemented_def = Define`
+  interference_implemented mc ffi_proj ms0 ⇔
+    ∃next_interfer ccache_interfer ffi_interfer.
+    (∀n. mc.next_interfer n = next_interfer) ∧
+    (∀n. mc.ccache_interfer n = ccache_interfer) ∧
+    (∀n. mc.ffi_interfer n = ffi_interfer) ∧
+    ∀ms k0. (ms = FUNPOW mc.target.next k0 ms0) ⇒
+      (mc.target.get_pc ms ∈ mc.prog_addresses ⇒
+        ∃k. (next_interfer (mc.target.next ms)
+             = FUNPOW mc.target.next k (mc.target.next ms)) ∧
+            (ffi_proj ms = ffi_proj (mc.target.next ms)) ∧
+            (ffi_proj (mc.target.next ms) =
+             ffi_proj (FUNPOW mc.target.next k (mc.target.next ms)))) ∧
+      ((mc.target.get_pc ms = mc.ccache_pc) ⇒
+        ∃k. (ccache_interfer
+             (mc.target.get_reg ms mc.ptr_reg,
+              mc.target.get_reg ms mc.len_reg,ms)
+             = FUNPOW mc.target.next k ms) ∧
+            (ffi_proj ms =
+             ffi_proj (FUNPOW mc.target.next k ms))) ∧
+        ∀ffi_index bytes bytes2 new_ffi new_bytes.
+          (find_index (mc.target.get_pc ms) mc.ffi_entry_pcs 0 = SOME ffi_index) ∧
+          (read_ffi ms mc = (SOME bytes, SOME bytes2)) ∧
+          (call_FFI (ffi_proj ms) (EL ffi_index mc.ffi_names) bytes bytes2 =
+            FFI_return new_ffi new_bytes)
+          ⇒
+          ∃k.
+            (ffi_interfer (ffi_index,new_bytes,ms) =
+             FUNPOW mc.target.next k ms) ∧
+            (ffi_proj (FUNPOW mc.target.next k ms) = new_ffi)`;
 
 val evaluate_Halt_FUNPOW_next = Q.store_thm("evaluate_Halt_FUNPOW_next",
   `∀mc ffi k ms t ms' ffi'.
-   interfer_FUNPOW_next record_ffi mc ms ∧
+   interference_implemented mc ffi_proj ms ∧
+   (ffi_proj ms = ffi) ∧
    (evaluate mc ffi k ms = (Halt t, ms', ffi')) ⇒
      ∃k'. (ms' = FUNPOW mc.target.next k' ms) ∧
-          (record_ffi ms ffi.io_events ⇒
-           record_ffi ms' ffi'.io_events)`,
-  rewrite_tac[interfer_FUNPOW_next_def]
-  \\ ho_match_mp_tac targetSemTheory.evaluate_ind
+          (ffi_proj ms' = ffi')`,
+  ho_match_mp_tac targetSemTheory.evaluate_ind
   \\ rpt gen_tac
   \\ strip_tac
   \\ rpt gen_tac
@@ -156,54 +160,49 @@ val evaluate_Halt_FUNPOW_next = Q.store_thm("evaluate_Halt_FUNPOW_next",
     last_x_assum mp_tac
     \\ impl_tac
     >- (
-      conj_tac >- (
-        rw[]
-        \\ last_assum(qspecl_then[`0`,`0`]mp_tac)
-        \\ strip_tac \\ fs[GSYM FUNPOW_ADD]
-        \\ last_x_assum(qspecl_then[`n+1`,`k'+k''+1`]mp_tac)
-        \\ rw[])
+      fs[interference_implemented_def]
       \\ conj_tac >- (
-        rw[]
-        \\ last_x_assum(qspecl_then[`0`,`0`]strip_assume_tac)
+        qx_gen_tac`k0`
+        \\ first_assum(qspec_then`0`(mp_tac o CONJUNCT1))
+        \\ impl_tac >- fs[]
+        \\ disch_then(qx_choose_then`k1`strip_assume_tac)
         \\ fs[GSYM FUNPOW_ADD]
-        \\ last_x_assum(qspecl_then[`n`,`k'+k''+1`]mp_tac)
-        \\ rw[])
-      \\ rw[]
-      \\ last_x_assum(qspecl_then[`0`,`0`]strip_assume_tac)
-      \\ fs[GSYM FUNPOW_ADD]
-      \\ last_x_assum(qspecl_then[`n`,`i`,`b`,`k'+k''+1`]strip_assume_tac)
-      \\ fs[GSYM FUNPOW_ADD]
-      \\ qexists_tac`k'''` \\ fs[])
-    \\ rw[]
-    \\ last_x_assum(qspecl_then[`0`,`0`]strip_assume_tac)
-    \\ fs[GSYM FUNPOW_ADD] \\ rw[]
-    \\ qexists_tac`k'+k''+1` \\ rw[])
+        \\ first_x_assum(qspec_then`SUC(k0+k1)`mp_tac)
+        \\ simp[FUNPOW] \\ strip_tac
+        \\ rw[] \\ fs[ADD1,FUNPOW_ADD]
+        \\ metis_tac[])
+      \\ first_x_assum(qspec_then`0`mp_tac)
+      \\ simp[] \\ rw[] \\ fs[] )
+    \\ disch_then(qx_choose_then`k1`strip_assume_tac)
+    \\ fs[interference_implemented_def]
+    \\ first_x_assum(qspec_then`0`(mp_tac o CONJUNCT1))
+    \\ simp[]
+    \\ disch_then(qx_choose_then`k2`strip_assume_tac)
+    \\ fs[GSYM FUNPOW_ADD]
+    \\ qexists_tac`k1+k2+1` \\ rw[FUNPOW_ADD] )
   >- (
     last_x_assum mp_tac
     \\ impl_tac
     >- (
       conj_tac >- (
-        rw[]
-        \\ qpat_assum`!n k. ?k'. _`(qspecl_then[`0`,`0`]strip_assume_tac)
-        \\ fs[GSYM FUNPOW_ADD]
-        \\ last_x_assum(qspecl_then[`n`,`k'+k''`]mp_tac)
-        \\ rw[])
-      \\ conj_tac >- (
-        rw[]
-        \\ qpat_assum`!n k. ?k'. _`(qspecl_then[`0`,`0`]strip_assume_tac)
-        \\ fs[GSYM FUNPOW_ADD]
-        \\ qpat_x_assum`∀n k. ?k'. _`(qspecl_then[`n+1`,`k'+k''`]mp_tac)
-        \\ rw[])
-      \\ rw[]
-      \\ qpat_assum`!n k. ?k'. _`(qspecl_then[`0`,`0`]strip_assume_tac)
-      \\ fs[GSYM FUNPOW_ADD]
-      \\ last_x_assum(qspecl_then[`n`,`i`,`b`,`k'+k''`]strip_assume_tac)
-      \\ fs[GSYM FUNPOW_ADD]
-      \\ qexists_tac`k'''` \\ fs[])
-    \\ qpat_assum`!n k. ?k'. _`(qspecl_then[`0`,`0`]strip_assume_tac)
+        fs[interference_implemented_def]
+        \\ qx_gen_tac`k0`
+        \\ first_assum(qspec_then`0`(mp_tac o CONJUNCT1 o CONJUNCT2))
+        \\ impl_tac >- fs[]
+        \\ disch_then(qx_choose_then`k1`strip_assume_tac)
+        \\ fs[GSYM FUNPOW_ADD])
+      \\ fs[interference_implemented_def]
+      \\ first_x_assum(qspec_then`0`(mp_tac o CONJUNCT1 o CONJUNCT2))
+      \\ simp[]
+      \\ disch_then(qx_choose_then`k1`strip_assume_tac)
+      \\ fs[GSYM FUNPOW_ADD])
+    \\ disch_then(qx_choose_then`k1`strip_assume_tac)
+    \\ fs[interference_implemented_def]
+    \\ first_x_assum(qspec_then`0`(mp_tac o CONJUNCT1 o CONJUNCT2))
+    \\ simp[]
+    \\ disch_then(qx_choose_then`k2`strip_assume_tac)
     \\ fs[GSYM FUNPOW_ADD]
-    \\ rw[]
-    \\ qexists_tac`k'+k''` \\ rw[])
+    \\ qexists_tac`k1+k2` \\ rw[])
   >- (
     fs[CaseEq"option"]
     \\ reverse(fs[CaseEq"ffi$ffi_result"]) \\ rfs[]
@@ -213,40 +212,39 @@ val evaluate_Halt_FUNPOW_next = Q.store_thm("evaluate_Halt_FUNPOW_next",
     \\ impl_tac
     >- (
       conj_tac >- (
-        rw[]
-        \\ first_assum(qspecl_then[`0`,`ffi_index`,`new_bytes`,`0`]strip_assume_tac)
-        \\ fs[GSYM FUNPOW_ADD]
-        \\ last_x_assum(qspecl_then[`n`,`k'+k''`]mp_tac)
-        \\ rw[])
-      \\ conj_tac >- (
-        rw[]
-        \\ last_assum(qspecl_then[`0`,`ffi_index`,`new_bytes`,`0`]strip_assume_tac)
-        \\ fs[GSYM FUNPOW_ADD]
-        \\ qpat_x_assum`∀n k. ?k'. _`(qspecl_then[`n`,`k'+k''`]mp_tac)
-        \\ rw[])
-      \\ rw[]
-      \\ last_assum(qspecl_then[`0`,`ffi_index`,`new_bytes`,`0`]strip_assume_tac)
-      \\ fs[GSYM FUNPOW_ADD]
-      \\ last_x_assum(qspecl_then[`n+1`,`i`,`b`,`k'+k''`]strip_assume_tac)
-      \\ fs[GSYM FUNPOW_ADD]
-      \\ qexists_tac`k'''` \\ fs[])
-    \\ rw[]
-    \\ first_assum(qspecl_then[`0`,`ffi_index`,`new_bytes`,`0`]strip_assume_tac)
+        fs[interference_implemented_def]
+        \\ qx_gen_tac`k0`
+        \\ first_assum(qspec_then`0`(mp_tac o CONJUNCT2 o CONJUNCT2))
+        \\ simp_tac(srw_ss())[]
+        \\ disch_then drule
+        \\ disch_then drule
+        \\ disch_then drule
+        \\ disch_then drule
+        \\ disch_then(qx_choose_then`k1`strip_assume_tac)
+        \\ fs[GSYM FUNPOW_ADD])
+      \\ fs[interference_implemented_def]
+      \\ first_x_assum(qspec_then`0`(mp_tac o CONJUNCT2 o CONJUNCT2))
+      \\ simp[]
+      \\ disch_then(qx_choose_then`k1`strip_assume_tac)
+      \\ fs[GSYM FUNPOW_ADD])
+    \\ disch_then(qx_choose_then`k1`strip_assume_tac)
+    \\ fs[interference_implemented_def]
+    \\ first_x_assum(qspec_then`0`(mp_tac o CONJUNCT2 o CONJUNCT2))
+    \\ simp[]
+    \\ disch_then(qx_choose_then`k2`strip_assume_tac)
     \\ fs[GSYM FUNPOW_ADD]
-    \\ qexists_tac`k'+k''` \\ rw[]
-    \\ first_x_assum match_mp_tac
-    \\ rfs[]
-    \\ fs[ffiTheory.call_FFI_def]
-    \\ fs[CaseEq"bool",CaseEq"oracle_result"] \\ rw[] \\ rfs[]));
+    \\ qexists_tac`k1+k2` \\ rw[]));
 
+(*
 val machine_sem_Terminate_FUNPOW_next = Q.store_thm("machine_sem_Terminate_FUNPOW_next",
-  `interfer_FUNPOW_next record_ffi mc ms ∧
-   record_ffi ms st.io_events ∧
+  `interference_implemented mc ffi_proj ms ∧
+   (ffi_proj ms = st.io_events) ∧
    machine_sem mc st ms (Terminate t io_events) ⇒
-   ∃k. record_ffi (nxt mc k ms) io_events`,
+   ∃k. ffi_proj (nxt mc k ms) = io_events`,
   rw[targetSemTheory.machine_sem_def]
   \\ imp_res_tac evaluate_Halt_FUNPOW_next
   \\ rfs[] \\ metis_tac[]);
+*)
 
 val ALIGNED_eq_aligned = Q.store_thm("ALIGNED_eq_aligned",
   `ALIGNED = aligned 2`,
@@ -1829,22 +1827,6 @@ val extract_print_from_mem_get_print_string = Q.store_thm("extract_print_from_me
   \\ simp[o_DEF,ADD1,GSYM word_add_n2w]);
 
 (*
-val ag32_record_ffi_def = Define`
-  ag32_record_ffi r0 ms ls ⇔
-    (MAP (extract_print_from_mem print_string_max_length r0) ms.io_events
-     = MAP (λx. case x of IO_event _ conf _ => MAP (CHR o w2n) conf) ls)`;
-
-interfer_FUNPOW_next is too strong...
-
-val interfer_FUNPOW_next_ag32_record_ffi = Q.store_thm("interfer_FUNPOW_next_ag32_record_ffi",
-  `interfer_FUNPOW_next (ag32_record_ffi r0) (hello_machine_config r0) (hello_init_ag32_state r0)`,
-  simp[interfer_FUNPOW_next_def]
-  \\ conj_tac
-  >- (
-    rw[hello_machine_config_def]
-    \\ qexists_tac`0` \\ simp[]
-*)
-
 val hello_ag32_next = Q.store_thm("hello_ag32_next",
   `byte_aligned r0 ∧ w2n r0 + memory_size < dimword (:32) ⇒
    ∃k. let ms = FUNPOW Next k (ag32_init_state (hello_init_memory r0) r0) in
@@ -1862,5 +1844,6 @@ val hello_ag32_next = Q.store_thm("hello_ag32_next",
   \\ rw[]
   \\ first_x_assum(mp_then Any mp_tac (GEN_ALL machine_sem_Terminate_FUNPOW_next))
   \\ cheat);
+*)
 
 val _ = export_theory();
